patch files generated by Isabelle using GNU ed

src/Syntax/Digraph.thy
@@ -3,39 +3,41 @@ theory Digraph
     Main
     "HOL-Library.Predicate_Compile_Alternative_Defs"
     HOL.Complete_Lattices
+    "HOL-Data_Structures.Tree_Set"
+    "HOL-Data_Structures.Tree_Map"
+    (* "HOL-Data_Structures.HOL-Library.Tree" *)
 begin
 
-record 'a digraph =
-  vertices :: \<open>'a set\<close>
-  edges :: \<open>'a \<rightharpoonup> 'a set\<close>
+definition fold_set :: \<open>('a \<Rightarrow> 'b \<Rightarrow> 'b) \<Rightarrow> 'b \<Rightarrow> 'a tree \<Rightarrow> 'b\<close>
+where \<open>fold_set f x t \<equiv> List.fold f (preorder t) x\<close>
 
-definition empty :: \<open>'a digraph\<close>
-where \<open>empty = \<lparr> vertices = {}, edges = Map.empty \<rparr>\<close>
+record ('a :: linorder) digraph =
+  vertices :: \<open>'a tree\<close>
+  edges :: \<open>('a \<times> 'a tree) tree\<close>
 
-lemma finite_empty: \<open>finite (vertices empty)\<close>
-  by (simp add: empty_def)
+definition empty :: \<open>('a :: linorder) digraph\<close>
+where \<open>empty = \<lparr> vertices = \<langle>\<rangle>, edges = \<langle>\<rangle> \<rparr>\<close>
 
 hide_const (open) empty
 
-definition add_vert :: \<open>'a \<Rightarrow> 'a digraph \<Rightarrow> 'a digraph\<close>
-where \<open>add_vert x g \<equiv> \<lparr> vertices = {x} \<union> vertices g, edges = edges g \<rparr>\<close>
+definition add_vert :: \<open>('a :: linorder) \<Rightarrow> 'a digraph \<Rightarrow> 'a digraph\<close>
+where \<open>add_vert x g \<equiv> \<lparr> vertices = Tree_Set.insert x (vertices g), edges = edges g \<rparr>\<close>
 
-lemma finite_add_vert: \<open>finite (vertices G) \<Longrightarrow> finite (vertices (add_vert x G))\<close>
-  by (simp add: add_vert_def)
+definition add_edge :: \<open>('a :: linorder) \<times> 'a \<Rightarrow> 'a digraph \<Rightarrow> 'a digraph\<close>
+where \<open>add_edge x g \<equiv> (
+         let (a, b) = x in
+         \<lparr> vertices = Tree_Set.insert a (Tree_Set.insert b (vertices g)),
+           edges = case Tree_Map.lookup (edges g) a of
+             None \<Rightarrow> Tree_Map.update a (Tree_Set.insert b \<langle>\<rangle>) (edges g)
+           | Some es \<Rightarrow> Tree_Map.update a (Tree_Set.insert b es) (edges g) \<rparr>)\<close>
 
-definition add_edge :: \<open>'a \<times> 'a \<Rightarrow> 'a digraph \<Rightarrow> 'a digraph\<close>
-where \<open>add_edge x g \<equiv> (let (a, b) = x in \<lparr> vertices = {a, b} \<union> vertices g, edges = (edges g)(a \<mapsto> {b} \<union> case_option {} id (edges g a)) \<rparr>)\<close>
-
-lemma finite_add_edge: \<open>finite (vertices G) \<Longrightarrow> finite (vertices (add_edge (x, y) G))\<close>
-  by (simp add: add_edge_def)
-
-definition has_vertex :: \<open>'a \<Rightarrow> 'a digraph \<Rightarrow> bool\<close>
-where \<open>has_vertex x g \<equiv> x \<in> vertices g\<close>
+definition has_vertex :: \<open>('a :: linorder) \<Rightarrow> 'a digraph \<Rightarrow> bool\<close>
+where \<open>has_vertex x g \<equiv> isin (vertices g) x\<close>
 
 lemma has_vertex_empty: \<open>has_vertex x Digraph.empty \<longleftrightarrow> False\<close>
   by (simp add: has_vertex_def empty_def)
 
-lemma has_vertex_add_vert: \<open>has_vertex x (add_vert x G)\<close>
+(* lemma has_vertex_add_vert: \<open>has_vertex x (add_vert x G)\<close>
   by (simp add: has_vertex_def add_vert_def)
 
 lemma has_vertex_add_vert2: \<open>x \<noteq> y \<Longrightarrow> has_vertex x (add_vert y G) \<Longrightarrow> has_vertex x G\<close>
@@ -48,46 +50,39 @@ lemma has_vertex_add_edge_proj2: \<open>has_vertex x (add_edge (y, x) G)\<close>
   by (simp add: has_vertex_def add_edge_def)
 
 lemma has_vertex_add_edge2: \<open>x \<noteq> y \<Longrightarrow> x \<noteq> z \<Longrightarrow> has_vertex x (add_edge (y, z) G) \<Longrightarrow> has_vertex x G\<close>
-  by (simp add: has_vertex_def add_edge_def)
+  by (simp add: has_vertex_def add_edge_def) *)
 
-definition postset :: \<open>'a \<Rightarrow> 'a digraph \<Rightarrow> 'a set\<close>
-where \<open>postset x g \<equiv> {y. y \<in> the (edges g x)}\<close>
+definition postset :: \<open>('a :: linorder) \<Rightarrow> 'a digraph \<Rightarrow> 'a tree\<close>
+where \<open>postset x g \<equiv> case Tree_Map.lookup (edges g) x of
+         None \<Rightarrow> \<langle>\<rangle>
+       | Some es \<Rightarrow> fold_set (\<lambda>y s. if isin es y then Tree_Set.insert y s else s) \<langle>\<rangle> (vertices g)\<close>
 
-lemma postset_empty: \<open>postset x Digraph.empty = {}\<close>
+lemma postset_empty: \<open>postset x Digraph.empty = \<langle>\<rangle>\<close>
   sorry
 
-lemma postset_add_vert_empty: \<open>postset x (add_vert y Digraph.empty) = {}\<close>
+lemma postset_add_vert_empty: \<open>postset x (add_vert y Digraph.empty) = \<langle>\<rangle>\<close>
   sorry
 
-lemma finite_postset: \<open>finite (vertices G) \<Longrightarrow> \<forall>x \<in> vertices G. finite (postset x G)\<close>
-  sorry
-
-definition preset :: \<open>'a \<Rightarrow> 'a digraph \<Rightarrow> 'a set\<close>
-where \<open>preset x g \<equiv> {y. x \<in> the (edges g y)}\<close>
-
-lemma finite_preset: \<open>finite (vertices G) \<Longrightarrow> \<forall>x \<in> vertices G. finite (preset x G)\<close>
-  sorry
+definition preset :: \<open>('a :: linorder) \<Rightarrow> 'a digraph \<Rightarrow> 'a tree\<close>
+where \<open>preset x g \<equiv> fold_set (\<lambda>y s. case Tree_Map.lookup (edges g) y of
+                                      None \<Rightarrow> s
+                                    | Some es \<Rightarrow> if isin es x then Tree_Set.insert y s else s) \<langle>\<rangle> (vertices g)\<close>
 
 text \<open>
   Returns \<open>Inr sort\<close> when the graph could be fully walked without finding cycles (\<open>sort\<close> is the associated topsort).
   Returns \<open>Inl cycle\<close> where \<open>cycle\<close> is the first cycle found in the graph.
 \<close>
-function walk_aux1 :: \<open>'a \<Rightarrow> 'a digraph \<Rightarrow> 'a list \<Rightarrow> 'a list + 'a list\<close>
-     and walk_aux2 :: \<open>'a digraph \<Rightarrow> 'a list + 'a list \<Rightarrow> 'a set \<Rightarrow> 'a list + 'a list\<close>
-where \<open>walk_aux1 root g stack = walk_aux2 g (Inr stack) (postset root g)\<close>
+function walk_aux1 :: \<open>('a :: linorder) \<Rightarrow> 'a digraph \<Rightarrow> 'a list \<Rightarrow> 'a list + 'a list\<close>
+     and walk_aux2 :: \<open>'a digraph \<Rightarrow> 'a \<Rightarrow> 'a list + 'a list \<Rightarrow> 'a list + 'a list\<close>
+where \<open>walk_aux1 root g stack = fold_set (walk_aux2 g) (Inr stack) (postset root g)\<close>
 
-    | \<open>walk_aux2 g (Inl cycle) _ = Inl cycle\<close>
-    | \<open>walk_aux2 g (Inr stack) vs = (
-         if Set.is_empty vs
-         then Inr stack
-         else
-           let v = Inf vs in
-           let vs = vs - {v} in
-           if v \<in> set stack
-           then Inl (v # stack)
-           else case walk_aux1 v g (v # stack) of
-             Inl cycle \<Rightarrow> Inl cycle
-           | Inr stack' \<Rightarrow> walk_aux2 g (Inr (List.remdups (stack @ stack'))) vs
+    | \<open>walk_aux2 g _ (Inl cycle) = Inl cycle\<close>
+    | \<open>walk_aux2 g v (Inr stack) = (
+         if List.member stack v
+         then Inl (v # stack)
+         else case walk_aux1 v g (v # stack) of
+           Inl cycle \<Rightarrow> Inl cycle
+         | Inr stack' \<Rightarrow> Inr (List.remdups (stack @ stack'))
        )\<close>
 by pat_completeness auto
 (* FIXME: Somehow \<open>Inf vs\<close> requires \<open>'a :: Inf\<close> *)
@@ -105,7 +100,7 @@ code_pred Finite_Set.fold_graph .
   apply simp
   sorry *)
 
-definition walk :: \<open>'a \<Rightarrow> 'a digraph \<Rightarrow> 'a list + 'a list\<close>
+definition walk :: \<open>('a :: linorder) \<Rightarrow> 'a digraph \<Rightarrow> 'a list + 'a list\<close>
 where \<open>walk x g \<equiv> walk_aux1 x g [x]\<close>
 
 lemma walk_empty_graph: \<open>walk x Digraph.empty = Inr [x]\<close>
@@ -118,10 +113,12 @@ text \<open>
   Tries to apply a topological sort on the directed graph (any root).
   The result is a left value containing a cycle if there is one, otherwise a right value with the full sort.
 \<close>
-fun topsort :: \<open>'a digraph \<Rightarrow> 'a list + 'a list\<close>
-where \<open>topsort g = walk (SOME x. x \<in> vertices g) g\<close>
+definition topsort :: \<open>('a :: linorder) digraph \<Rightarrow> 'a list + 'a list\<close>
+where \<open>topsort g \<equiv> case vertices g of
+         \<langle>\<rangle> \<Rightarrow> Inr []
+       | \<langle>_, x, _\<rangle> \<Rightarrow> walk x g\<close>
 
-definition has_cycle_from :: \<open>'a \<Rightarrow> 'a digraph \<Rightarrow> 'a list option\<close>
+definition has_cycle_from :: \<open>('a :: linorder) \<Rightarrow> 'a digraph \<Rightarrow> 'a list option\<close>
 where \<open>has_cycle_from x g \<equiv> case_sum Some (\<lambda>_. None) (walk x g)\<close>
 
 lemma no_cycle_empty_graph: \<open>has_cycle_from x Digraph.empty = None\<close>
@@ -134,5 +131,7 @@ lemma no_cycle_singleton: \<open>has_cycle_from x (add_vert x Digraph.empty) = N
 
 lemma has_cycle_topsort: \<open>has_cycle_from x G = Some c1 \<Longrightarrow> \<exists>c2. topsort G = Inl c2\<close>
   sorry
+
+hide_const fold_set
 
 end
