app/EntryPoint.thy
@@ -31,15 +31,15 @@ where \<open>add_all_files \<equiv> List.fold (\<lambda>(a, b) d. add_file d a b
 
 (* TODO: add files to diagnostic *)
 
-fun go_typecheck :: \<open>(String.literal \<rightharpoonup> AST.module located) \<Rightarrow> String.literal list list \<Rightarrow> unit io\<close>
+fun go_typecheck :: \<open>(String.literal \<times> AST.module located) tree \<Rightarrow> String.literal list list \<Rightarrow> unit io\<close>
 where \<open>go_typecheck asts mods = IO.return ()\<close>
 
 term run_driver
 
 fun entrypoint :: \<open>all_flags \<Rightarrow> unit io\<close>
 where \<open>entrypoint (AllFlags input output) = do {
-         (result, (names, files)) \<leftarrow> run_driver input;
-         let files = List.map (\<lambda>n. (n, the (files n))) (List.remdups names);
+         (result, files) \<leftarrow> run_driver input;
+         let files = inorder files;
          case result of
            Inl diag \<Rightarrow> print_diagnostic_and_quit (add_all_files files diag)
          | Inr (asts, mods) \<Rightarrow> go_typecheck asts mods
