src/Syntax/Driver.thy
@@ -14,7 +14,7 @@ theory Driver
     CLI.Flags
 begin
 
-fun run_driver :: \<open>input_flags \<Rightarrow> ((String.literal diagnostic + (String.literal \<rightharpoonup> AST.module located) \<times> module_order) \<times> registered_files) io\<close>
+fun run_driver :: \<open>input_flags \<Rightarrow> ((String.literal diagnostic + (String.literal \<times> AST.module located) tree \<times> module_order) \<times> registered_files) io\<close>
 where \<open>run_driver (InputFlags idirs mods) = do {
          parse_and_resolve_modules idirs mods;
          IO.return undefined
